SimpleRef: Work on preservation

proof/DDC/Language/SimpleRef/Preservation.v
@@ -3,28 +3,68 @@ Require Import DDC.Language.SimpleRef.Step.
 Require Import DDC.Language.SimpleRef.SubstExpExp.
 Require Import DDC.Language.SimpleRef.Ty.
 
+Definition extends (ys: stenv) (xs: stenv)
+ := exists zs, ys = zs >< xs.
+
+Lemma type_stenv_extends
+ : forall te se1 se2 x t1
+ ,  extends se2 se1
+ -> TYPE te se1 x t1
+ -> TYPE te se2 x t1.
+Proof.
+ intros.
+ simpl in H.
+ destruct H as [se3]. subst.
+ auto.
+Qed.
+Hint Resolve type_stenv_extends.
+
 
 (* If a closed, well typed expression takes an evaluation step 
    then the result has the same type as before. *)
 Theorem preservation
- :  forall x x' t
- ,  TYPE nil x  t
- -> STEP x x'
- -> TYPE nil x' t.
+ :  forall se h x h' x' t
+ ,  TYPEH se h
+ -> TYPE  nil se x  t
+ -> STEP  h x h' x'
+ -> (exists se', extends se' se /\ TYPE  nil se' x' t /\ TYPEH se' h').
 Proof.
- intros. gen t.
- induction H0; intros.
+ intros se h x h' x' t HTH HT HS. gen t.
+ induction HS; intros.
 
  Case "EsContext".
-  destruct H.
-  eauto.
-  inverts H1. eauto.
-  inverts H1. eauto.
+  specializes IHHS HTH.
+  destruct H; try
+   (inverts HT;
+    edestruct IHHS as [se2]; eauto;
+    exists se2;
+    splits; try tauto;
+    repeat (match goal with 
+     | [ H : _ /\ _ |- _ ] => inverts H
+    end); eauto).
 
  Case "EsLamApp".
-  inverts H0.
+  inverts HT.
   inverts H4.
+  exists se. splits; auto.
+   admit. (* extends is wrong *)
   eapply subst_exp_exp; eauto.
+
+ Case "EsLamNewRef".
+  inverts HT.
+  exists (tData <: se). splits.
+   admit. (* extends is wrong *)
+   eapply TyLoc.
+    admit. (* ok, list lemma *)
+    admit. (* ok *)   
+
+ Case "EsReadRef".
+  inverts HT.
+  inverts H3.
+  exists se. splits.
+  admit. (* extends *)
+  admit. (* ok *)
+  auto.
 Qed.
 
 
